Allow calls to side-effect-free ghost methods from expressions

Source/Dafny/DafnyAst.cs
@@ -4715,6 +4715,8 @@ namespace Microsoft.Dafny {
       } else if (S is CalcStmt) {
         var s = (CalcStmt)S;
         return s.Result;
+      } else if (S is UpdateStmt) {
+        return new LiteralExpr(tok, true);  // one could use the postcondition of the method, suitably instantiated, but "true" is conservative and much simpler :)
       } else {
         Contract.Assert(false); throw new cce.UnreachableException();  // unexpected statement
       }
